more slow progress on compiler correctness
Made force_dom take a default value so that we can still know something
good about the values in the environments stored in closures in badly
typed terms.

Tried fixing EVERY_Cexp to be more (mutually) recursive, but termination
proofs become impossible. Instead, made it easy to automatically define
instances of EVERY_Cexp P from the interesting equations for P (i.e.
automatically fill out the recursion).

Fixed semantics of Cevaluate for calling recursive closures: was putting
the index rather than the name as the last component of the CRecClos
generated for the environment in which to evaluate the body. Also need
to canonicalise the environment for those CRecClos's. But now thinking
perhaps it would be better to simply check closures have good
environments everywhere in Cevaluate, and also force good environments
for anything it produces... i.e. move the proof of that fact into the
definition.

examples/miniML/compiler/compileCorrectnessScript.sml
@@ -175,6 +175,7 @@ val i0_def = CompileTheory.i0_def
 val Cevaluate_ind = CompileTheory.Cevaluate_ind
 val Cevaluate_strongind = CompileTheory.Cevaluate_strongind
 val mk_env_def = CompileTheory.mk_env_def
+val find_index_def = CompileTheory.find_index_def
 
 val (Cevaluate_list_with_rules,Cevaluate_list_with_ind,Cevaluate_list_with_cases) = Hol_reln [ANTIQUOTE(
 Cevaluate_rules |> SIMP_RULE (srw_ss()) [] |> concl |>
@@ -662,6 +663,20 @@ rw[FOLDL2_FOLDL,MAP2_MAP,ZIP_MAP,MAP_ZIP,LENGTH_ZIP,
    pairTheory.UNCURRY,pairTheory.LAMBDA_PROD,FUPDATE_LIST,
    rich_listTheory.FOLDL_MAP])
 
+val SND_FOLDL2_FUPDATE_LIST = store_thm(
+"SND_FOLDL2_FUPDATE_LIST",
+``!f1 f2 bs cs a n. (LENGTH bs = LENGTH cs) ⇒
+  (SND (FOLDL2 (λ(n,fm) b c. (n + 1, fm |+ (f1 n b c, f2 n b c))) (n,a) bs cs) =
+   let ns = GENLIST ($+ n) (LENGTH cs) in
+   a |++ ZIP (MAP2 (UNCURRY f1) (ZIP (ns,bs)) cs, MAP2 (UNCURRY f2) (ZIP (ns,bs)) cs))``,
+ntac 2 gen_tac >>
+Induct >- rw[LENGTH_NIL,LENGTH_NIL_SYM,LET_THM,FUPDATE_LIST_THM] >>
+gen_tac >> Cases >> rw[LET_THM] >>
+fs[FUPDATE_LIST_THM,LET_THM,GENLIST_CONS] >>
+`$+ n o SUC = $+ (n + 1)` by (
+  srw_tac[ARITH_ss][FUN_EQ_THM] ) >>
+rw[])
+
 val UNCURRY_K_I_o_FST = store_thm(
 "UNCURRY_K_I_o_FST",
 ``UNCURRY K = I o FST``,
@@ -682,15 +697,14 @@ rw[INJ_DEF])
 val mk_env_canon = store_thm(
 "mk_env_canon",
 ``!(env1:num|->Cv) env2 exp ns. (mk_env env1 exp ns = mk_env env2 exp ns) =
-  (∀x. x ∈ free_vars exp DIFF ns ⇒ (env1 ' x = env2 ' x))``,
+  (∀x. x ∈ free_vars exp DIFF ns ⇒ ((env1 ⊌ (FEMPTY|+(x,CLit(Bool F)))) ' x = (env2 ⊌ (FEMPTY|+(x,CLit(Bool F)))) ' x))``,
 rw[mk_env_def,sort_Cenv_def] >>
 rw[num_Cv_linear_order_linear,QSORT_eq_if_PERM,PERM_fmap_to_alist,
-   fsetTheory.force_dom_def,GSYM fmap_EQ_THM] >>
-rw[FUN_FMAP_DEF])
+   fsetTheory.force_dom_def,GSYM fmap_EQ_THM,FUNION_DEF,FUN_FMAP_DEF])
 
 val force_dom_DRESTRICT_FUNION = store_thm(
 "force_dom_DRESTRICT_FUNION",
-``FINITE s ⇒ (force_dom fm s = (DRESTRICT fm s ⊌ (FUN_FMAP ($FAPPLY FEMPTY) s)))``,
+``FINITE s ⇒ (force_dom fm s d = (DRESTRICT fm s ⊌ (FUN_FMAP (K d) s)))``,
 rw[fsetTheory.force_dom_def,GSYM fmap_EQ_THM,DRESTRICT_DEF,FUN_FMAP_DEF,FUNION_DEF] >>
 rw[EXTENSION,EQ_IMP_THM,NOT_FDOM_FAPPLY_FEMPTY])
 
@@ -758,6 +772,8 @@ MAP_ZIP
 |> SIMP_RULE (srw_ss()) [f pairTheory.FST,f pairTheory.SND]
 end
 
+val Cexp_size_def = CompileTheory.Cexp_size_def
+
 fun mk_EVERY ty = let
   val (name,_) = dest_type ty
   val EVERY_ty = "EVERY_"^name
@@ -787,8 +803,6 @@ fun mk_EVERY ty = let
   val eqs = map eq args
 in [ANTIQUOTE (list_mk_conj eqs)] end
 
-val tys = [``:Cexp``,``:Cv``]
-
 val variant_args = let
   fun f (x,(vs,acc)) = let val v = with_flag (Globals.priming,SOME"") (variant vs) x in (v::vs,v::acc) end
   fun g (tm,(vs,acc)) = let
@@ -809,12 +823,12 @@ let val ty' = type_of tm in
 let val ty'' = listSyntax.dest_list_type ty' in
 let val (tya,tyb) = pairSyntax.dest_prod ty'' in
 let
-  fun f p EVP = listfn(uneta EVP,listSyntax.mk_map(inst[alpha|->tya,beta|->tyb]p,tm))
+  fun f p EVP = listfn((*uneta*) EVP,listSyntax.mk_map(inst[alpha|->tya,beta|->tyb]p,tm))
   val acc = add (f pairSyntax.fst_tm) tya acc
   val acc = add (f pairSyntax.snd_tm) tyb acc
 in acc end
 end handle HOL_ERR {origin_function="dest_prod",...} =>
-  add (fn EVP => listfn(uneta EVP,tm)) ty'' acc
+  add (fn EVP => listfn((*uneta*) EVP,tm)) ty'' acc
 end handle HOL_ERR {origin_function="dest_list_type",...} =>
   add (fn EVP => mk_comb(EVP,tm)) ty' acc
 end
@@ -854,7 +868,8 @@ fun mk_EVERY cvtr tys = let
       val EV = List.nth(EVERY_tys,j)
       val P = List.nth(Ps,j)
       val EVP = mk_comb(EV,P)
-      val EVP = if i = j then EVP else mk_comb(cvtr j i,EVP)
+      val EVP = if i = j then EVP
+        else mk_comb(List.nth(EVERY_tys,i),uneta(mk_comb(cvtr j i,uneta EVP)))
       in f EVP :: acc end
   fun eq tm = let
     val ty = type_of tm
@@ -864,9 +879,10 @@ fun mk_EVERY cvtr tys = let
   in
     mk_eq(list_mk_comb(EVERY_ty,[P,tm]),list_mk_conj((mk_comb(P,tm))::(foldl (find_tys listSyntax.mk_every (add i)) [] (#2(strip_comb tm)))))
   end
-  val eqs = map (fn args => list_mk_conj (map eq args)) argss
-in map ANTIQUOTE eqs end
+  val eqs = list_mk_conj (map eq (rev (flatten argss)))
+in [ANTIQUOTE eqs] end
 
+(*
 val EVERY_Cbody_def = Define (mk_every_cvtr "EVERY_Cbody" ``:Cexp`` ``:Cv``)
 val EVERY_CVal_def = Define (mk_every_cvtr "EVERY_CVal" ``:Cv`` ``:Cexp``)
 val EXISTS_Cbody_def = Define (mk_exists_cvtr "EXISTS_Cbody" ``:Cexp`` ``:Cv``)
@@ -897,10 +913,32 @@ fs[EVERY_MEM,EXISTS_MEM] >>
 metis_tac[])
 val _ = DefnBase.export_cong"EVERY_CVal_cong"
 
-val [EVERY_Cv_eqs,EVERY_Cexp_eqs] = mk_EVERY cvtr [``:Cexp``,``:Cv``]
+val EVERY_Cexp_eqs = mk_EVERY cvtr [``:Cexp``,``:Cv``]
 
-val Cexp_size_def = CompileTheory.Cexp_size_def
+val _ = Hol_datatype`
+  ty1 = C1 | C2 of ty2 ;
+  ty2 = D1 of ty1`
+val foo_def = xDefine "foo"`
+  (foo P C1 = P C1) /\
+  (foo P (C2 t2) = bar (\x. foo P x) t2) /\
+  (bar P (D1 t1) = foo P t1)`
+val foo_def = xDefine "foo"`
+  (foo f P C1 = P C1) /\
+  (foo f P (C2 t2) = f (\x. foo f P x) t2)`
 
+val EVERY_Cexp_def = tDefine "EVERY_Cexp" EVERY_Cexp_eqs(
+WF_REL_TAC `inv_image $< (λx. case x of | INR (_,v) => Cv_size v | INL (_,e) => Cexp_size e)` >>
+srw_tac[ARITH_ss][Cexp3_size_thm,Cexp8_size_thm,Cexp7_size_thm,Cexp4_size_thm,Cexp1_size_thm] >>
+Q.ISPEC_THEN `Cv_size` imp_res_tac SUM_MAP_MEM_bound >>
+Q.ISPEC_THEN `Cexp_size` imp_res_tac SUM_MAP_MEM_bound >>
+fsrw_tac[ARITH_ss][Cexp_size_def,SUM_MAP_Cexp2_size_thm,SUM_MAP_Cexp6_size_thm,SUM_MAP_Cexp5_size_thm] >>
+TRY (qmatch_assum_rename_tac `EXISTS_CVal X yy` ["X"]) >>
+TRY (qmatch_assum_rename_tac `EXISTS_Cbody X yy` ["X"]) >>
+Cases_on`yy`>>fs[]
+impossible because of mutual nested recursion
+*)
+
+(*
 val EVERY_Cv_def = tDefine "EVERY_Cv" [EVERY_Cv_eqs](
 WF_REL_TAC `measure (Cv_size o SND)` >>
 srw_tac[ARITH_ss][Cexp3_size_thm,Cexp8_size_thm] >>
@@ -911,6 +949,8 @@ Cases_on`cv`>>fs[]>>rw[]>>
 fsrw_tac[ARITH_ss][Cexp_size_def,Cexp1_size_thm,SUM_MAP_Cexp2_size_thm] >>
 Q.ISPEC_THEN `Cexp_size` imp_res_tac SUM_MAP_MEM_bound >>
 fsrw_tac[ARITH_ss][Cexp_size_def])
+val EVERY_Cv_thm = save_thm(
+"EVERY_Cv_thm",SIMP_RULE((srw_ss())++boolSimps.ETA_ss)[]EVERY_Cv_def)
 
 val EVERY_Cexp_def = tDefine "EVERY_Cexp" [EVERY_Cexp_eqs](
 WF_REL_TAC `measure (Cexp_size o SND)` >>
@@ -922,17 +962,60 @@ Cases_on`ll`>>fs[]>>rw[Cexp_size_def,Cexp3_size_thm,Cexp1_size_thm,SUM_MAP_Cexp2
 fs[EXISTS_MEM] >>
 Q.ISPEC_THEN `Cexp_size` imp_res_tac SUM_MAP_MEM_bound >>
 fsrw_tac[ARITH_ss][Cexp_size_def])
+val EVERY_Cexp_thm = save_thm(
+"EVERY_Cexp_thm",SIMP_RULE((srw_ss())++boolSimps.ETA_ss)[]EVERY_Cexp_def)
 
-val _ = export_rewrites["EVERY_Cv_def","EVERY_Cexp_def"]
+val _ = export_rewrites["EVERY_Cv_thm","EVERY_Cexp_thm"]
+*)
 
-val canonical_env_def = Define`
-  (canonical_env (CClosure env ns b) = (FDOM (alist_to_fmap env) = free_vars b DIFF (set ns))) ∧
-  (canonical_env (CRecClos env ns bs n) = case find_index n ns 0 of
-    SOME i => (FDOM (alist_to_fmap env) = free_vars (SND (EL i bs)) DIFF (set (FST (EL i bs))) DIFF (set ns))
-    | NONE => F) ∧
-  (canonical_env _ = T)`
+fun mk_EVERY name eqns tys = let
+  val tynames = map (#1 o dest_type) tys
+  val foo_tys = map (fn n => name^"_"^n) tynames
+  val foo_tys = map (fn (foo_ty,ty) => mk_var(foo_ty,ty-->bool)) (zip foo_tys tys)
+  val argss = map args_from_nchotomy tys
+  val lrs = map (((#2 o dest_comb) ## I) o dest_eq) eqns
+  val lhss = map fst lrs
+  val avoids = mk_set (foo_tys@(flatten (map (#2 o strip_comb) lhss)))
+  fun h (tms,(vs,acc)) = let
+    val (vs,tms) = foldl variant_args (vs,[]) tms
+  in (vs,tms::acc) end
+  val (_,argss) = foldl h (avoids,[]) argss
+  val argss = map (fn args => map (fn t => case total (first (can (match_term t))) lhss of SOME l => l | NONE => t) args) argss
+  fun add f ty acc =
+    case total (index (equal ty)) tys of
+      NONE => acc
+    | SOME i => f (List.nth(foo_tys,i)) :: acc
+  fun eq tm = let
+    val ty = type_of tm
+    val i = index (equal ty) tys
+    val foo_ty = List.nth(foo_tys,i)
+    val rhsl = case total (first ((equal tm) o #1)) lrs of NONE => [] | SOME (_,r) => [r]
+    val rhs = lmk_conj(rev(foldl (find_tys listSyntax.mk_every add) rhsl (#2(strip_comb tm))))
+  in
+    mk_eq(mk_comb(foo_ty,tm),rhs)
+  end
+  val eqs = list_mk_conj (map eq (rev (flatten argss)))
+in [ANTIQUOTE eqs] end
 
-val _ = export_rewrites["canonical_env_def"]
+val canonical_env_eqs = mk_EVERY
+"canonical_env"
+[(``canonical_env (CClosure env ns b) = (FDOM (alist_to_fmap env) = free_vars b DIFF (set ns))``),
+ (``canonical_env (CRecClos env ns bs n) =
+    case find_index n ns 0 of
+      SOME i => (FDOM (alist_to_fmap env) = free_vars (SND (EL i bs)) DIFF (set (FST (EL i bs))) DIFF (set ns))
+    | NONE => F``)]
+[``:Cexp``,``:Cv``]
+
+val canonical_env_def = tDefine "canonical_env" canonical_env_eqs(
+WF_REL_TAC `inv_image $< (λx. case x of | INR v => Cv_size v | INL e => Cexp_size e)` >>
+srw_tac[ARITH_ss][Cexp3_size_thm,Cexp8_size_thm,Cexp7_size_thm,Cexp4_size_thm,Cexp1_size_thm] >>
+Q.ISPEC_THEN `Cv_size` imp_res_tac SUM_MAP_MEM_bound >>
+Q.ISPEC_THEN `Cexp_size` imp_res_tac SUM_MAP_MEM_bound >>
+fsrw_tac[ARITH_ss][Cexp_size_def,SUM_MAP_Cexp2_size_thm,SUM_MAP_Cexp6_size_thm,SUM_MAP_Cexp5_size_thm])
+val canonical_env_thm = save_thm(
+"canonical_env_thm",SIMP_RULE((srw_ss())++boolSimps.ETA_ss)[]canonical_env_def)
+
+val _ = export_rewrites["canonical_env_thm"]
 
 val FOLDL2_Cmatch_bind_error = store_thm(
 "FOLDL2_Cmatch_bind_error",
@@ -944,18 +1027,16 @@ gen_tac >> Cases >> rw[])
 
 val Cpmatch_canonical_envs = store_thm(
 "Cpmatch_canonical_envs",
-``(∀env p v env'. (Cpmatch env p v = Cmatch env') ∧ (∀v. v ∈ FRANGE env ⇒ EVERY_Cv canonical_env v) ∧ EVERY_Cv canonical_env v ⇒ (∀v. v ∈ FRANGE env' ⇒ EVERY_Cv canonical_env v)) ∧
-(∀env ps vs env'. (Cpmatch_list env ps vs = Cmatch env') ∧ (∀v. v ∈ FRANGE env ⇒ EVERY_Cv canonical_env v) ∧ EVERY (EVERY_Cv canonical_env) vs ⇒ (∀v. v ∈ FRANGE env' ⇒ EVERY_Cv canonical_env v))``,
+``(∀env p v env'. (Cpmatch env p v = Cmatch env') ∧ (∀v. v ∈ FRANGE env ⇒ canonical_env_Cv v) ∧ canonical_env_Cv v ⇒ (∀v. v ∈ FRANGE env' ⇒ canonical_env_Cv v)) ∧
+(∀env ps vs env'. (Cpmatch_list env ps vs = Cmatch env') ∧ (∀v. v ∈ FRANGE env ⇒ canonical_env_Cv v) ∧ EVERY canonical_env_Cv vs ⇒ (∀v. v ∈ FRANGE env' ⇒ canonical_env_Cv v))``,
 ho_match_mp_tac Cpmatch_ind >>
 rw[Cpmatch_def] >>
-fs[FRANGE_DEF] >> rw[DOMSUB_FAPPLY_THM] >>
-(ASSUM_LIST (fn ls => if length ls < 7 then NO_TAC else ALL_TAC)
- ORELSE metis_tac[]) >>
+fs[FRANGE_DEF] >> rw[DOMSUB_FAPPLY_THM]
+>- metis_tac[] >>
 Cases_on `Cpmatch env p v` >> fs[] >>
 qmatch_assum_rename_tac `Cpmatch env p v = Cmatch env''` [] >>
 first_x_assum (qspecl_then [`env''`,`env'`] (match_mp_tac o MP_CANON)) >>
-rw[] >>
-metis_tac[])
+rw[] >> metis_tac[])
 
 val FST_triple = store_thm(
 "FST_triple",
@@ -965,6 +1046,21 @@ rw[FUN_EQ_THM,pairTheory.UNCURRY])
 val SND_triple = store_thm(
 "SND_triple",
 ``(λ(n,ns,b). f ns b) = UNCURRY f o SND``,
+rw[FUN_EQ_THM,pairTheory.UNCURRY])
+
+val FST_pair = store_thm(
+"FST_pair",
+``(λ(n,v). n) = FST``,
+rw[FUN_EQ_THM,pairTheory.UNCURRY])
+
+val SND_pair = store_thm(
+"SND_pair",
+``(λ(n,v). v) = SND``,
+rw[FUN_EQ_THM,pairTheory.UNCURRY])
+
+val SND_FST_pair = store_thm(
+"SND_FST_pair",
+``(λ((n,m),c).m) = SND o FST``,
 rw[FUN_EQ_THM,pairTheory.UNCURRY])
 
 val MEM_QSORT = store_thm(
@@ -979,18 +1075,88 @@ val MEM_sort_Cenv = store_thm(
 rw[sort_Cenv_def])
 val _ = export_rewrites["MEM_sort_Cenv"]
 
-val EVERY_Cexp_EVERY_CVal_imp = store_thm(
-"EVERY_Cexp_EVERY_CVal_imp",
-``∀P e. EVERY_Cexp (EVERY_CVal P) e ⇒ EVERY_CVal P e``,
-gen_tac >> Cases >> rw[])
+val LENGTH_QSORT = store_thm(
+"LENGTH_QSORT",
+``LENGTH (QSORT R ls) = LENGTH ls``,
+METIS_TAC[QSORT_PERM,PERM_LENGTH])
+val _ = export_rewrites["LENGTH_QSORT"]
+
+val LENGTH_sort_Cenv = store_thm(
+"LENGTH_sort_Cenv",
+``LENGTH (sort_Cenv env) = LENGTH env``,
+rw[sort_Cenv_def])
+val _ = export_rewrites["LENGTH_sort_Cenv"]
+
+val set_MAP_QSORT = store_thm(
+"set_MAP_QSORT",
+``set (MAP f (QSORT R ls)) = set (MAP f ls)``,
+METIS_TAC[QSORT_PERM,PERM_LIST_TO_SET,PERM_MAP])
+val _ = export_rewrites["set_MAP_QSORT"]
+
+val set_MAP_sort_Cenv = store_thm(
+"set_MAP_sort_Cenv",
+``set (MAP f (sort_Cenv env)) = set (MAP f env)``,
+rw[sort_Cenv_def])
+val _ = export_rewrites["set_MAP_sort_Cenv"]
+
+val EVERY_QSORT = store_thm(
+"EVERY_QSORT",
+``EVERY P (QSORT R ls) = EVERY P ls``,
+METIS_TAC[QSORT_PERM,EVERY_MEM,MEM_PERM])
+val _ = export_rewrites["EVERY_QSORT"]
+
+val EVERY_sort_Cenv = store_thm(
+"EVERY_sort_Cenv",
+``EVERY P (sort_Cenv env) = EVERY P env``,
+rw[sort_Cenv_def])
+val _ = export_rewrites["EVERY_sort_Cenv"]
+
+val FDOM_force_dom = store_thm(
+"FDOM_force_dom",
+``∀s env d. FINITE s ⇒ (FDOM (force_dom env s d) = s)``,
+rw[force_dom_DRESTRICT_FUNION,FDOM_DRESTRICT] >>
+rw[EXTENSION] >> metis_tac[])
+val _ = export_rewrites["FDOM_force_dom"]
+
+val find_index_ALL_DISTINCT_EL = store_thm(
+"find_index_ALL_DISTINCT_EL",
+``∀ls n m. ALL_DISTINCT ls ∧ n < LENGTH ls ⇒ (find_index (EL n ls) ls m = SOME (m + n))``,
+Induct >- rw[] >>
+gen_tac >> Cases >>
+srw_tac[ARITH_ss][find_index_def] >>
+metis_tac[MEM_EL])
+val _ = export_rewrites["find_index_ALL_DISTINCT_EL"]
+
+val find_index_LESS_LENGTH = store_thm(
+"find_index_LESS_LENGTH",
+``∀ls n m i. (find_index n ls m = SOME i) ⇒ (i < m + LENGTH ls)``,
+Induct >> rw[find_index_def] >>
+res_tac >>
+srw_tac[ARITH_ss][arithmeticTheory.ADD1])
+
+val set_MAP_FST_fmap_to_alist = store_thm(
+"set_MAP_FST_fmap_to_alist",
+``set (MAP FST (fmap_to_alist fm)) = FDOM fm``,
+METIS_TAC[fmap_to_alist_to_fmap,FDOM_alist_to_fmap])
+val _ = export_rewrites["set_MAP_FST_fmap_to_alist"]
+
+val DIFF_UNION = store_thm(
+"DIFF_UNION",
+``!x y z. x DIFF (y UNION z) = x DIFF y DIFF z``,
+SRW_TAC[][EXTENSION] THEN METIS_TAC[])
+
+val DIFF_COMM = store_thm(
+"DIFF_COMM",
+``!x y z. x DIFF y DIFF z = x DIFF z DIFF y``,
+SRW_TAC[][EXTENSION] THEN METIS_TAC[])
 
 (*
 val Cevaluate_canonical_envs = store_thm(
 "Cevaluate_canonical_envs",
 ``∀env exp res. Cevaluate env exp res ⇒
-  ((∀v. v ∈ FRANGE env ⇒ EVERY_Cv canonical_env v) ∧
-   (EVERY_Cexp (EVERY_CVal (EVERY_Cv canonical_env)) exp))
-⇒ ∀v. (res = Rval v) ⇒ EVERY_Cv canonical_env v``,
+  ((∀v. v ∈ FRANGE env ⇒ canonical_env_Cv v) ∧
+   canonical_env_Cexp exp)
+⇒ ∀v. (res = Rval v) ⇒ canonical_env_Cv v``,
 ho_match_mp_tac Cevaluate_nice_ind >> rw[] >>
 TRY (
   first_x_assum match_mp_tac >>
@@ -1004,9 +1170,9 @@ TRY (
   metis_tac[] ) >>
 TRY (
   pop_assum mp_tac >> rw[] >>
-  `EVERY_Cv canonical_env (env ' n)` by (
+  `canonical_env_Cv (env ' n)` by (
     fs[FRANGE_DEF] >> metis_tac[] ) >>
-  `∀v. v ∈ FRANGE env' ⇒ EVERY_Cv canonical_env v` by
+  `∀v. v ∈ FRANGE env' ⇒ canonical_env_Cv v` by
     imp_res_tac Cpmatch_canonical_envs >>
   fs[] ) >>
 TRY (
@@ -1014,7 +1180,7 @@ TRY (
   rw[] >> fs[] >>
   first_x_assum match_mp_tac >>
   fs[FRANGE_DEF] >> rw[DOMSUB_FAPPLY_THM] >>
-  metis_tac[])
+  metis_tac[]) >>
 TRY (
   pop_assum match_mp_tac >>
   fs[FOLDL2_FUPDATE_LIST_paired] >>
@@ -1030,24 +1196,112 @@ TRY (
       qpat_assum `LENGTH ns = LENGTH defs` assume_tac >> fs[] >>
       rw[EL_MAP,Abbr`ls`,Abbr`P`,MAP_ZIP,LENGTH_ZIP,EL_ZIP] >>
       rw[pairTheory.UNCURRY] >- (
-        rw[EXTENSION,MEM_MAP,mk_env_def,pairTheory.EXISTS_PROD,FLOOKUP_DEF] )
+        rw[EXTENSION,MEM_MAP,mk_env_def,pairTheory.EXISTS_PROD,FLOOKUP_DEF]  >>
+        metis_tac[])
       >- (
-        fsrw_tac[boolSimps.ETA_ss][EVERY_MAP,EVERY_MEM,MEM_EL] >>
-        metis_tac[EVERY_Cexp_EVERY_CVal_imp] ) >>
-      fsrw_tac[boolSimps.ETA_ss][EVERY_MAP,mk_env_def,EVERY_MEM,pairTheory.FORALL_PROD,FLOOKUP_DEF,force_dom_DRESTRICT_FUNION,FUNION_DEF,DRESTRICT_DEF] >>
-      rw[] >> fs[]
-      )
-      rw[EL_MAP]
-
+        fsrw_tac[boolSimps.ETA_ss][EVERY_MAP,mk_env_def,EVERY_MEM,pairTheory.FORALL_PROD,FLOOKUP_DEF,force_dom_DRESTRICT_FUNION,FUNION_DEF,DRESTRICT_DEF] >>
+        rw[] >> fs[] >>
+        fsrw_tac[SATISFY_ss][FUN_FMAP_DEF]) >>
+      fsrw_tac[boolSimps.ETA_ss][EVERY_MAP,EVERY_MEM,MEM_EL] >>
+      metis_tac[]) >>
+    rw[EL_MAP,Abbr`ls`,LENGTH_ZIP,MAP_ZIP] >>
+    match_mp_tac FUPDATE_LIST_APPLY_MEM >>
+    qexists_tac `n` >>
+    qpat_assum `LENGTH ns = LENGTH defs` assume_tac >> fs[] >>
+    rw[LENGTH_ZIP,MAP_ZIP] >>
+    fs[EL_ALL_DISTINCT_EL_EQ] >>
+    srw_tac[ARITH_ss][] ) >>
+  fs[] >> rw[] >>
+  qmatch_abbrev_tac `P ((env |++ ls) ' x)` >>
+  qsuff_tac `(env |++ ls) ' x = env ' x` >- ( rw[Abbr`P`] ) >>
+  match_mp_tac FUPDATE_LIST_APPLY_NOT_MEM >>
+  unabbrev_all_tac >>
+  rw[MAP_ZIP,LENGTH_ZIP] ) >>
+TRY (
+  fs[EXTENSION,MEM_MAP,mk_env_def,pairTheory.EXISTS_PROD,FLOOKUP_DEF] >>
+  metis_tac[] ) >>
+TRY (
+  fs[EVERY_MEM,MEM_MAP,pairTheory.EXISTS_PROD,mk_env_def,FLOOKUP_DEF,force_dom_DRESTRICT_FUNION,FUNION_DEF,DRESTRICT_DEF] >>
+  rw[] >>
+  srw_tac[SATISFY_ss][FUN_FMAP_DEF] >>
+  fs[FRANGE_DEF] >> metis_tac[] ) >>
+TRY (
+  fs[] >>
+  pop_assum match_mp_tac >>
+  fs[FOLDL2_FUPDATE_LIST,MAP2_MAP,FST_pair,SND_pair,MAP_ZIP,FRANGE_DEF,FDOM_FUPDATE_LIST,EVERY_MEM,MEM_MAP,pairTheory.EXISTS_PROD] >>
+  rw[] >- (
+    qmatch_abbrev_tac `canonical_env_Cv ((env1 |++ ls) ' x)` >>
+    qsuff_tac `(env1 |++ ls) ' x = env1 ' x` >- (
+      unabbrev_all_tac >> rw[] >>
+      qmatch_rename_tac `canonical_env_Cv (alist_to_fmap al ' x)` [] >>
+      `∃v. (ALOOKUP al x = SOME v)` by (
+        rw[ALOOKUP_LEAST_EL] >>
+        REWRITE_TAC[GSYM IN_LIST_TO_SET] >>
+        ASM_REWRITE_TAC[] >>
+        rw[] ) >>
+      imp_res_tac ALOOKUP_MEM >>
+      metis_tac[ALOOKUP_SOME_FAPPLY_alist_to_fmap] ) >>
+    match_mp_tac FUPDATE_LIST_APPLY_NOT_MEM_matchable >>
+    rw[Abbr`ls`,MAP_ZIP] ) >>
+  fs[MEM_EL] >>
+  qmatch_abbrev_tac `canonical_env_Cv ((env1 |++ ZIP (ns,vs)) ' (EL n ns))` >>
+  qsuff_tac `(env1 |++ ZIP (ns,vs)) ' (EL n ns) = EL n vs` >- (
+    rw[] >> fs[Cevaluate_list_with_value] >>
+    metis_tac[] ) >>
+  match_mp_tac FUPDATE_LIST_APPLY_MEM >>
+  rw[LENGTH_ZIP,EL_MAP,MAP_ZIP,EL_ZIP] >>
+  qexists_tac `n` >> rw[] >>
+  fs[EL_ALL_DISTINCT_EL_EQ] >>
+  srw_tac[ARITH_ss][] ) >>
+TRY (
+  fs[] >>
+  pop_assum match_mp_tac >>
+  fs[Cevaluate_list_with_value] >>
+  fs[FOLDL2_FUPDATE_LIST,FOLDL2_FUPDATE_LIST_paired,MAP2_MAP,FST_pair,SND_pair,MAP_ZIP,FRANGE_DEF,FDOM_FUPDATE_LIST,EVERY_MEM,MEM_MAP,pairTheory.EXISTS_PROD,LENGTH_ZIP,LET_THM,MEM_ZIP] >>
+  reverse conj_tac >- metis_tac[MEM_EL,find_index_LESS_LENGTH,arithmeticTheory.ADD_0,arithmeticTheory.ADD_SYM] >>
+  qx_gen_tac `v` >>
+  fs[GSYM LEFT_FORALL_IMP_THM] >>
+  qx_gen_tac `x` >>
+  Cases_on `MEM x ns` >> fs[] >- (
+    fs[MEM_EL] >>
+    qmatch_abbrev_tac `((env1 |++ ls) ' (EL n1 ns) = v) ⇒ P` >>
+    qsuff_tac `(env1 |++ ls) ' (EL n1 ns) = EL n1 vs` >- (
       rw[Abbr`P`] >> metis_tac[] ) >>
-    match_mp_tac FUPDATE_LIST_APPLY_NOT_MEM >>
-    unabbrev_all_tac >>
-    rw[MAP_ZIP,LENGTH_ZIP]
-    fs[FUPDATE_LIST_APPLY_NOT_MEM,MAP_ZIP,LENGTH_ZIP]
+    match_mp_tac FUPDATE_LIST_APPLY_MEM >>
+    rw[Abbr`ls`,LENGTH_ZIP,EL_MAP,MAP_ZIP,EL_ZIP] >>
+    qexists_tac `n1` >> srw_tac[ARITH_ss][] >>
+    fs[EL_ALL_DISTINCT_EL_EQ] >>
+    srw_tac[ARITH_ss][] ) >>
+  Cases_on `MEM x ns'` >> fs[] >- (
+    qmatch_abbrev_tac `Q ∧ ((env1 |++ ls) ' x = v) ⇒ P` >>
+    qsuff_tac `(env1 |++ ls) ' x = env1 ' x` >- (
+      unabbrev_all_tac >> rw[] >>
+      fs[MEM_EL] >>
+      qho_match_abbrev_tac `P ((env1 |++ (ZIP (l1,l2))) ' (EL n1 ns'))` >>
+      qsuff_tac `((env1 |++ (ZIP (l1,l2))) ' (EL n1 l1)) = EL n1 l2` >- (
+        unabbrev_all_tac >>
+        qpat_assum `LENGTH ns' = LENGTH defs` assume_tac >>
+        qpat_assum `ALL_DISTINCT ns'` assume_tac >> fs[] >>
+        fs[EL_MAP,LENGTH_ZIP,LENGTH_GENLIST,EL_ZIP,EVERY_MEM,MEM_MAP,find_index_ALL_DISTINCT_EL,MAP_ZIP,FST_triple] >>
+        disch_then kall_tac >>
+        qpat_assum `(e1 |++ ls) ' X = e1 ' X` kall_tac >>
+        fs[pairTheory.UNCURRY,mk_env_def,EVERY_MAP,DIFF_UNION,DIFF_COMM] >>
+        reverse conj_tac >- (
+          rw[EVERY_MEM,MEM_EL,pairTheory.LAMBDA_PROD,pairTheory.FORALL_PROD] >>
+          metis_tac[] ) >>
+        fs[EVERY_MEM,pairTheory.FORALL_PROD,FLOOKUP_DEF] >>
+        rw[force_dom_DRESTRICT_FUNION,FUNION_DEF,DRESTRICT_DEF,FUN_FMAP_DEF] >>
+        qmatch_rename_tac `canonical_env_Cv (alist_to_fmap env' ' x)` [] >>
+        qsuff_tac `∃v. ALOOKUP env' x = SOME v` >- (
+          rw[] >>
+          imp_res_tac ALOOKUP_SOME_FAPPLY_alist_to_fmap >>
+          fs[ALOOKUP_LEAST_EL] >>
+
+val sorry:tactic = (fn (asl,g) => ([],K(mk_thm([],g))))
 
 val Cevaluate_any_env = store_thm(
 "Cevaluate_any_env",
-``∀env exp res. Cevaluate env exp res ⇒ ∀env'. Cevaluate ((force_dom env (free_vars exp)) ⊌ env') exp res``,
+``∀env exp res. Cevaluate env exp res ⇒ ∀env'. Cevaluate ((force_dom env (free_vars exp) (CLit(Bool F))) ⊌ env') exp res``,
 fs[force_dom_DRESTRICT_FUNION] >>
 ho_match_mp_tac Cevaluate_nice_ind >>
 rw[FOLDL_UNION_BIGUNION,FOLDL_UNION_BIGUNION_paired,
@@ -1063,7 +1317,7 @@ TRY (
   qsuff_tac `env0 ⊌ env1 = env1` >- PROVE_TAC[] >>
   rw[GSYM SUBMAP_FUNION_ABSORPTION] >>
   rw[Abbr`env0`,Abbr`env1`,SUBMAP_DEF,DRESTRICT_DEF,FUNION_DEF,FUN_FMAP_DEF] >>
-  srw_tac[boolSimps.DNF_ss][FUN_FMAP_DEF] >>
+  srw_tac[boolSimps.DNF_ss,SATISFY_ss][FUN_FMAP_DEF] >>
   metis_tac[] ) >>
 TRY (
   fs[Once Cpmatch_FEMPTY] >>
@@ -1076,7 +1330,7 @@ TRY (
   rw[GSYM SUBMAP_FUNION_ABSORPTION] >>
   rw[Abbr`env0`,Abbr`env1`,SUBMAP_DEF,DRESTRICT_DEF,FUNION_DEF,FUN_FMAP_DEF,pairTheory.UNCURRY] >>
   srw_tac[boolSimps.DNF_ss][FUN_FMAP_DEF,pairTheory.UNCURRY] >>
-  fsrw_tac[boolSimps.DNF_ss][FUN_FMAP_DEF,pairTheory.UNCURRY] >>
+  fsrw_tac[boolSimps.DNF_ss,SATISFY_ss][FUN_FMAP_DEF,pairTheory.UNCURRY] >>
   metis_tac[] ) >>
 TRY (
   disj1_tac >>
@@ -1088,7 +1342,7 @@ TRY (
   rw[GSYM SUBMAP_FUNION_ABSORPTION] >>
   rw[Abbr`env0`,Abbr`env1`,Abbr`env2`,SUBMAP_DEF,DRESTRICT_DEF,FUNION_DEF,
      DRESTRICT_FUPDATE,FAPPLY_FUPDATE_THM,FUN_FMAP_DEF] >>
-  srw_tac[boolSimps.DNF_ss][FUN_FMAP_DEF] >>
+  srw_tac[boolSimps.DNF_ss,SATISFY_ss][FUN_FMAP_DEF] >>
   metis_tac[] ) >>
 TRY (
   disj2_tac >>
@@ -1098,7 +1352,7 @@ TRY (
   rw[GSYM SUBMAP_FUNION_ABSORPTION] >>
   rw[Abbr`env0`,Abbr`env1`,SUBMAP_DEF,DRESTRICT_DEF,FUNION_DEF,
      DRESTRICT_FUPDATE,FAPPLY_FUPDATE_THM] >>
-  srw_tac[boolSimps.DNF_ss][] >>
+  srw_tac[boolSimps.DNF_ss,SATISFY_ss][FUN_FMAP_DEF] >>
   metis_tac[] ) >>
 TRY (
   rw[Once Cevaluate_cases] >>
@@ -1145,12 +1399,15 @@ TRY (
       fs[EL_MAP,LENGTH_ZIP,EL_ZIP] >>
       rw[pairTheory.UNCURRY] >>
       rw[mk_env_canon] >>
-      qmatch_abbrev_tac `env ' x = (DRESTRICT env s ⊌ f0 ⊌ f2) ' x` >>
+      qmatch_abbrev_tac `(env ⊌ fF) ' x = ((DRESTRICT env s ⊌ f0 ⊌ f2) ⊌ fF) ' x` >>
       qsuff_tac `x ∈ s` >- (
         strip_tac >>
         Cases_on `x ∈ FDOM env` >>
-        rw[FUNION_DEF,DRESTRICT_DEF,Abbr`s`,NOT_FDOM_FAPPLY_FEMPTY] ) >>
-      unabbrev_all_tac >> rw[] >>
+        rw[FUNION_DEF,DRESTRICT_DEF,Abbr`s`,NOT_FDOM_FAPPLY_FEMPTY] >>
+        unabbrev_all_tac >>
+        srw_tac[SATISFY_ss][FUN_FMAP_DEF]) >>
+      unabbrev_all_tac >>
+      srw_tac[SATISFY_ss][FUN_FMAP_DEF] >>
       disj2_tac >>
       rw[pairTheory.UNCURRY] >>
       metis_tac[MEM_EL,IN_DIFF,IN_LIST_TO_SET,IN_UNION] ) >>
@@ -1166,15 +1423,18 @@ TRY (
    match_mp_tac EQ_SYM >>
    match_mp_tac FUPDATE_LIST_APPLY_NOT_MEM_matchable >>
    rw[MAP_ZIP,LENGTH_ZIP] >>
-   qmatch_abbrev_tac `FEMPTY ' x = (DRESTRICT env s ⊌ f0 ⊌ f2) ' x` >>
+   rw[FUN_FMAP_DEF] >>
+   qmatch_abbrev_tac `CLit (Bool F) = (DRESTRICT env s ⊌ f0 ⊌ f2) ' x` >>
    rw[DRESTRICT_DEF,FUNION_DEF,FUN_FMAP_DEF,Abbr`s`] ) >>
 TRY (
   rw[mk_env_canon] >>
-  qmatch_abbrev_tac `env ' x = (DRESTRICT env s ⊌ f0 ⊌ f2) ' x` >>
+  qmatch_abbrev_tac `(env ⊌ ff) ' x = ((DRESTRICT env s ⊌ f0 ⊌ f2) ⊌ ff) ' x` >>
   qsuff_tac `x ∈ s` >- (
     strip_tac >>
     Cases_on `x ∈ FDOM env` >>
-    rw[FUNION_DEF,DRESTRICT_DEF,Abbr`s`,NOT_FDOM_FAPPLY_FEMPTY] ) >>
+    rw[FUNION_DEF,DRESTRICT_DEF,Abbr`s`,NOT_FDOM_FAPPLY_FEMPTY] >>
+    unabbrev_all_tac >>
+    srw_tac[][FUN_FMAP_DEF]) >>
   rw[Abbr`s`] ) >>
 TRY (
   rw[Once Cevaluate_cases] >>
@@ -1189,27 +1449,28 @@ TRY (
   unabbrev_all_tac >>
   qmatch_abbrev_tac `Cevaluate env1 exp1 res1` >>
   qmatch_assum_abbrev_tac `∀env''. Cevaluate (env0 ⊌ env'') exp1 res1` >>
-  TRY (
-    rw[MAP2_MAP,MAP_ZIP_unfolded,FDOM_FUPDATE_LIST,MEM_MAP,MEM_ZIP] >>
-  )
-  qsuff_tac `env0 ⊌ env1 = env1` >- metis_tac[] >>
-  rw[GSYM SUBMAP_FUNION_ABSORPTION] >>
-  rw[SUBMAP_DEF,Abbr`env0`,Abbr`env1`,DRESTRICT_DEF,FUN_FMAP_DEF,FUNION_DEF] >>
-  srw_tac[boolSimps.DNF_ss][FUN_FMAP_DEF,MEM_EL,FOLDL2_FUPDATE_LIST] >>
-  metis_tac[]
-  >- (
-    rw[Cevaluate_list_with_Cevaluate] >>
-    fs[Cevaluate_list_with_value] >>
-    qx_gen_tac `n` >> rw[] >>
-    first_x_assum (qspec_then `n` mp_tac) >> rw[] >>
-    unabbrev_all_tac >>
-    qmatch_assum_abbrev_tac `∀env'. Cevaluate (env0 ⊌ env') (EL n es) (Rval (EL n vs))` >>
-    qmatch_abbrev_tac `Cevaluate env1 (EL n es) (Rval (EL n vs))` >>
+  (( qunabbrev_tac `exp1` >>
+    qmatch_abbrev_tac `Cevaluate env1 exp' res1` >>
     qsuff_tac `env0 ⊌ env1 = env1` >- metis_tac[] >>
     rw[GSYM SUBMAP_FUNION_ABSORPTION] >>
-    rw[SUBMAP_DEF,Abbr`env0`,Abbr`env1`,DRESTRICT_DEF,FUN_FMAP_DEF,FUNION_DEF]
-    srw_tac[boolSimps.DNF_ss][FUN_FMAP_DEF,MEM_EL] >>
-    metis_tac[] ) >>
+    fs[SUBMAP_DEF] >>
+    qx_gen_tac `x` >>
+    qunabbrev_tac `env0` >>
+    fs[DRESTRICT_DEF] >>
+    qmatch_abbrev_tac `A /\ B \/ B ==> C` >>
+    qsuff_tac `B ==> C` >- metis_tac[] >>
+    unabbrev_all_tac >>
+    fs[FOLDL2_FUPDATE_LIST,MAP2_MAP,MAP_ZIP,FST_pair,SND_pair,FDOM_FUPDATE_LIST,MEM_MAP,pairTheory.EXISTS_PROD] >>
+    sorry
+    (* TODO *)
+   ) ORELSE (
+    qsuff_tac `env0 ⊌ env1 = env1` >- metis_tac[] >>
+    rw[GSYM SUBMAP_FUNION_ABSORPTION] >>
+    rw[SUBMAP_DEF,Abbr`env0`,Abbr`env1`,DRESTRICT_DEF,FUN_FMAP_DEF,FUNION_DEF] >>
+    srw_tac[boolSimps.DNF_ss,SATISFY_ss][FUN_FMAP_DEF,FOLDL2_FUPDATE_LIST] >>
+    srw_tac[boolSimps.DNF_ss,SATISFY_ss][FUN_FMAP_DEF] >>
+    metis_tac[MEM_EL]
+   )))
 
 >> PROVE_TAC[]
 *)
